New adequacy proof for proving a sequence of programs refines another (modulo one admit).
This version implicitly does some of the inductive reasoning that the framework
previously did using the abstraction relation. The benefit over the previous
version is that we do not have to drop out of the logic to state the
abstraction relation.

Still need to actually instantiate this general theorem to get an eaiser to use
version for ExMach examples to see that this all actually paid off, but the
commit was getting big enough as is.

src/CSL/Adequacy.v
@@ -41,57 +41,73 @@ Proof.
   iExists ∅. rewrite fmap_empty big_opM_empty. by iFrame.
 Qed.
 
+
 (* Program logic adequacy *)
+Definition adequate_internal {Σ} {OpT T} {Λ: Layer OpT} (s : stuckness)
+           (e1 : proc OpT T) (σ1 : Λ.(State)) (φ : T → Λ.(State) → iProp Σ) k : iProp Σ :=
+  ((∀ (n: nat) σ2 res,
+    ⌜ Λ.(exec_n) e1 n σ1 (Val σ2 res) ⌝ →
+    (Nat.iter (S k + S (S n)) (λ P, |==> ▷ P)%I (∃ v, ⌜ res = existT _ v ⌝ ∧ φ v σ2))) ∧
+  ((∀ (n: nat),
+     ⌜ s = NotStuck ⌝ →
+     ⌜ Λ.(exec_partial_n) e1 n σ1 Err ⌝ →
+     (▷^(S k + S (S n)) False))))%I.
+
 Record adequate {OpT T} {Λ: Layer OpT} (s : stuckness) (e1 : proc OpT T) (σ1 : Λ.(State))
     (φ : T → Λ.(State) → Prop) := {
-  adequate_result σ2 res :
+   adequate_result σ2 res :
     Λ.(exec) e1 σ1 (Val σ2 res) → ∃ v, res = existT _ v ∧ φ v σ2;
-  adequate_not_stuck :
-   s = NotStuck →
-   ¬ Λ.(exec_partial) e1 σ1 Err
-}.
+    adequate_not_stuck :
+    s = NotStuck → ¬ Λ.(exec_partial) e1 σ1 Err
+ }.
 
 (* Adequacy for execution with a recovery procedure *)
+Definition recv_adequate_internal {Σ} {OpT T R} {Λ: Layer OpT} (s : stuckness) (e1 : proc OpT T)
+       (rec: proc OpT R) (σ1 : Λ.(State))
+       (φ : T → Λ.(State) → iProp Σ) (φrec: Λ.(State) → iProp Σ) k :=
+  (* recv_adequate_internal_normal_result n σ2 res  : *)
+  ((∀ n σ2 res,
+    ⌜ Λ.(exec_n) e1 n σ1 (Val σ2 res) ⌝ →
+    (Nat.iter (S k + (S (S n))) (λ P, |==> ▷ P)%I (∃ v, ⌜ res = existT _ v ⌝ ∧ φ v σ2)))
+   ∧
+   (∀ n σ2 res, 
+    ⌜ Λ.(rexec_n) e1 rec n σ1 (Val σ2 res) ⌝ →
+    (Nat.iter (S k + (5 + n))) (λ P, |==> ▷ P)%I (φrec σ2))
+   ∧
+  ((∀ (n: nat),
+     ⌜ s = NotStuck ⌝ →
+     ⌜ Λ.(rexec_n) e1 rec n σ1 Err ⌝ →
+     (▷^(S k + (5 + n)) False))))%I.
+
 Record recv_adequate {OpT T R} {Λ: Layer OpT} (s : stuckness) (e1 : proc OpT T)
        (rec: proc OpT R) (σ1 : Λ.(State)) (φ : T → Λ.(State) → Prop) (φrec: Λ.(State) → Prop) := {
-  recv_adequate_normal_result σ2 res :
-    Λ.(exec) e1 σ1 (Val σ2 res) → ∃ v, res = existT _ v ∧ φ v σ2;
-  recv_adequate_result σ2 res :
-    Λ.(rexec) e1 (rec_singleton rec) σ1 (Val σ2 res) → φrec σ2;
-  recv_adequate_not_stuck :
-    s = NotStuck →
-    ¬ Λ.(rexec) e1 (rec_singleton rec) σ1 Err
-}.
+   recv_adequate_normal_result σ2 res :
+     Λ.(exec) e1 σ1 (Val σ2 res) → ∃ v, res = existT _ v ∧ φ v σ2;
+   recv_adequate_result σ2 res :
+     Λ.(rexec) e1 (rec_singleton rec) σ1 (Val σ2 res) → φrec σ2;
+   recv_adequate_not_stuck :
+     s = NotStuck →
+     ¬ Λ.(rexec) e1 (rec_singleton rec) σ1 Err
+ }.
 
-(*
-Theorem adequate_tp_safe {OpT T} {Λ: Layer OpT} (e1 : proc OpT T) t2 σ1 σ2 φ :
-  adequate NotStuck e1 σ1 φ →
-  Λ.(step ([e1], σ1) (t2, σ2) →
-  Forall (λ e, is_Some (to_val e)) t2 ∨ ∃ t3 σ3, step (t2, σ2) (t3, σ3).
-Proof.
-  intros Had ?.
-  destruct (decide (Forall (λ e, is_Some (to_val e)) t2)) as [|Ht2]; [by left|].
-  apply (not_Forall_Exists _), Exists_exists in Ht2; destruct Ht2 as (e2&?&He2).
-  destruct (adequate_not_stuck NotStuck e1 σ1 φ Had t2 σ2 e2) as [?|(e3&σ3&efs&?)];
-    rewrite ?eq_None_not_Some; auto.
-  { exfalso. eauto. }
-  destruct (elem_of_list_split t2 e2) as (t2'&t2''&->); auto.
-  right; exists (t2' ++ e3 :: t2'' ++ efs), σ3; econstructor; eauto.
-Qed.
-*)
+Record proc_seq_adequate {OpT T R} {Λ: Layer OpT} (s : stuckness) (es : proc_seq OpT T)
+       (rec: proc OpT R) (σ1 : Λ.(State)) (φ : T → Λ.(State) → Prop) (φrec: Λ.(State) → Prop) := {
+   proc_seq_adequate_normal_result σ2 res :
+     Λ.(proc_exec_seq) es (rec_singleton rec) σ1 (Val σ2 res) →
+     match res with
+     | Normal e => ∃ v, e = existT _ v ∧ φ v σ2
+     | Recovered _ => φrec σ2
+     end;
+   proc_seq_adequate_not_stuck :
+     s = NotStuck →
+     ¬ Λ.(proc_exec_seq) es (rec_singleton rec) σ1 Err
+ }.
 
 Section adequacy.
 Context {OpT: Type → Type}.
 Context `{Λ: Layer OpT}.
 Context `{irisG OpT Λ Σ}.
-(*
-Implicit Types e : expr Λ.
-*)
 Implicit Types P Q : iProp Σ.
-(*
-Implicit Types Φ : val Λ → iProp Σ.
-Implicit Types Φs : list (val Λ → iProp Σ).
-*)
 
 Notation world' E σ := (wsat ∗ ownE E ∗ state_interp σ)%I (only parsing).
 Notation world σ := (world' ⊤ σ) (only parsing).
@@ -154,6 +170,13 @@ Proof.
   - simpl. iIntros "Hiter". iMod "Hiter". iModIntro. iNext. iApply ("IH" with "HPQ Hiter").
 Qed.
 
+Lemma bupd_iter_le n1 n2 P :
+  n1 ≤ n2 → Nat.iter n1 (λ P, |==> ▷ P)%I P -∗ Nat.iter n2 (λ P, |==> ▷ P)%I P.
+Proof.
+  iIntros (Hle). induction Hle; auto.
+  - simpl. iIntros "Hiter". iModIntro. iNext.  iApply (IHHle with "Hiter").
+Qed.
+
 Lemma wptp_steps_state_inv {T} s n e1 t1 t2 σ1 σ2 Φ :
   bind_rep_n n (Λ.(exec_pool)) (existT T e1 :: t1) σ1 (Val σ2 t2) →
   world σ1 ∗ WP e1 @ s; ⊤ {{ Φ }} ∗ wptp s t1 ⊢
@@ -200,6 +223,19 @@ Proof.
   done.
 Qed.
 
+Lemma wptp_result' {T T'} s n e1 t1 v2' t2 σ1 σ2 φ :
+  bind_rep_n n (Λ.(exec_pool)) (existT T e1 :: t1) σ1 (Val σ2 (existT T' (of_val v2') :: t2)) →
+  world σ1 ∗ WP e1 @ s; ⊤ {{ v, ∀ σ, state_interp σ ={⊤,∅}=∗ φ v σ }} ∗ wptp s t1
+  ⊢ Nat.iter (S (S n)) (λ P, |==> ▷ P)%I (∃ v2, ⌜ existT T (@of_val OpT _ v2) = existT T' (@of_val OpT _ v2') ⌝ ∧ φ v2 σ2).
+Proof.
+  intros. rewrite wptp_steps // (Nat_iter_S_r ((S n))). iApply bupd_iter_mono.
+  iDestruct 1 as (e2 t2' ?) "((Hw & HE & Hσ) & H & _)"; simplify_eq.
+  assert (Ret v2' = e2) by eauto with *; subst.
+  iDestruct (wp_value_inv' with "H") as "H". rewrite uPred_fupd_eq.
+  iMod ("H" with "[$]") as ">(Hw & HE & H)".
+  iExists v2'. iMod ("H" with "Hσ [$]") as ">(_ & _ & ?)"; auto.
+Qed.
+
 Lemma wptp_safe {T T'} n (e1: proc OpT T) (e2: proc OpT T') t1 t2 σ1 σ2 Φ :
   bind_rep_n n (Λ.(exec_pool)) (existT T e1 :: t1) σ1 (Val σ2 t2) →
   existT T' e2 ∈ t2 →
@@ -228,58 +264,112 @@ Proof.
 Qed.
 End adequacy.
 
-Theorem wp_strong_adequacy {T} OpT Σ Λ `{invPreG Σ} s (e: proc OpT T) σ φ k:
+Theorem adequacy_int_to_ext {T} OpT Σ Λ s (e: proc OpT T) σ φ k:
+  adequate_internal (Σ := Σ) (Λ := Λ) s e σ (fun v σ => ⌜ φ v σ ⌝)%I k →
+  adequate s e σ φ.
+Proof.
+  intros Hinternal. split.
+  * intros ?? Hexec. apply exec_equiv_exec_n in Hexec as (n&?).
+    eapply (soundness (M:=iResUR Σ) _ (S k + S (S n))).
+    iDestruct Hinternal as "(Hres&_)".
+    iApply bupd_iter_laterN_mono; first by reflexivity; eauto.
+    iApply bupd_iter_mono; last first.
+    { iApply "Hres"; eauto. }
+    { eauto. }
+  * intros ? Hexec. apply exec_partial_equiv_exec_partial_n in Hexec as (n&?).
+    eapply (soundness (M:=iResUR Σ) _ (S k + S (S n))).
+    iDestruct Hinternal as "(_&Hnstuck)". iApply "Hnstuck"; eauto.
+Qed.
+
+Theorem recv_adequacy_int_to_ext {T R} OpT Σ Λ (e: proc OpT T) (rec: proc OpT R) σ φ φrec k:
+  recv_adequate_internal (Σ := Σ) (Λ := Λ) NotStuck e rec σ
+                         (fun v σ => ⌜ φ v σ ⌝)%I (fun σ => ⌜ φrec σ ⌝)%I k →
+  recv_adequate NotStuck e rec σ φ φrec.
+Proof.
+  intros Hinternal.
+  assert (¬ rexec Λ e (rec_singleton rec) σ Err).
+  { 
+    intros Hrexec.
+    apply rexec_equiv_rexec_n'_err in Hrexec as (n&?Hrexec);
+      last eapply crash_non_err.
+    eapply (soundness (M:=iResUR Σ) _ (S k + (5 + n))).
+    iDestruct Hinternal as "(_&Hnstuck)". iApply "Hnstuck"; eauto.
+  }
+  split; auto.
+  - intros ?? Hexec.
+    apply exec_equiv_exec_n in Hexec as (n&?).
+    eapply (soundness (M:=iResUR Σ) _ (S k + S (S n))).
+    iDestruct Hinternal as "(Hres&_&_)".
+    iApply bupd_iter_laterN_mono; first by reflexivity; eauto.
+    iApply bupd_iter_mono; last first.
+    { iApply "Hres"; eauto. }
+    { eauto. }
+  - intros ? [] Hexec.
+    apply rexec_equiv_rexec_n'_val in Hexec as (n&?); eauto using crash_non_err.
+    eapply (soundness (M:=iResUR Σ) _ (S k + (5 + n))).
+    iDestruct Hinternal as "(_&Hres&_)".
+    iApply bupd_iter_laterN_mono; first by reflexivity; eauto.
+    iApply bupd_iter_mono; last first.
+    { iApply "Hres"; eauto. }
+    { eauto. }
+Qed.
+
+Theorem wp_strong_adequacy_internal {T} OpT Σ Λ `{invPreG Σ} s (e: proc OpT T) σ φ k:
   (∀ `{Hinv : invG Σ},
      Nat.iter k (λ P, |==> ▷ P)%I (|={⊤}=> ∃ stateI : State Λ → iProp Σ,
        let _ : irisG OpT Λ Σ := IrisG _ _ _ Hinv stateI in
-       stateI σ ∗ WP e @ s; ⊤ {{ v, ∀ σ, stateI σ ={⊤,∅}=∗ ⌜φ v σ⌝ }})%I) →
-  adequate s e σ φ.
+       stateI σ ∗ WP e @ s; ⊤ {{ v, ∀ σ, stateI σ ={⊤,∅}=∗  φ v σ  }})%I) ⊢
+  adequate_internal s e σ φ k.
 Proof.
-  intros Hwp; split.
-  - intros σ' (T'&v') Hexec.
-    destruct Hexec as ([|(?&e')]&?&Hpartial&Hcheck).
-    { inversion Hcheck. }
-    destruct e'; inversion Hcheck; subst.
-    inversion H3; subst.
-    unfold exec_partial in Hpartial.
-    apply bind_star_inv_rep_n in Hpartial as (n&Hpartial).
-    assert (v' = v).
-    { eapply Eqdep.EqdepTheory.inj_pair2 in H1; eauto. }
-    subst.
-    cut (∃ v0 : T, existT T (@of_val OpT _ v0) = existT T' (of_val v) ∧ φ v0 σ').
-    { intros (vnew&?&?). exists vnew; split; auto. inversion H0. congruence. }
-    eapply (soundness (M:=iResUR Σ) _ (S k + S (S n))).
-    rewrite laterN_plus.
-    iApply bupd_iter_laterN_mono; first by reflexivity.
-    iMod wsat_alloc as (Hinv) "[Hw HE]". specialize (Hwp _).
+  iIntros "Hwp"; iSplit.
+  - iIntros (n σ' (T'&v') Hexec).
+    destruct Hexec as (tp&Hpartial).
+    subst. simpl.
+    rewrite Nat_iter_add.
+    iMod wsat_alloc as (Hinv) "[Hw HE]". iSpecialize ("Hwp" $! _).
     iModIntro. iNext.
-    iApply (bupd_iter_mono k with "[Hw HE] []"); last by iApply Hwp.
+    iApply (bupd_iter_mono k with "[Hw HE] [Hwp]"); last by iApply "Hwp".
     iIntros "Hwp". rewrite {1}uPred_fupd_eq.
     iMod ("Hwp" with "[$Hw $HE]") as ">(Hw & HE & Hwp)".
     iDestruct "Hwp" as (Istate) "[HI Hwp]".
-    iApply (@wptp_result _ _ _ (IrisG _ _ _ Hinv Istate)); eauto with iFrame.
+    iPoseProof (@wptp_result' _ _ _ (IrisG _ _ _ Hinv Istate) with "[-]") as "H".
+    { eauto. }
+    { iFrame. rewrite //=. }
+    iApply (bupd_iter_mono (S (S n)) with "[] H").
+    iIntros "H". iDestruct "H" as (v'' Heq) "?". inversion Heq; subst.
+    iExists v''; iSplit; auto.
   - destruct s; last done.
-    intros _ Hpartial.
-    unfold exec_partial in Hpartial.
-    apply bind_star_inv_rep_n in Hpartial as (n&Hpartial).
+    iIntros (n ? Hpartial).
     assert (bind_rep_r_n n (exec_pool Λ) [existT T e] σ Err) as Hpartial_r.
     { apply bind_rep_lr_n in Hpartial. intuition. }
     apply bind_rep_r_n_err_inv in Hpartial_r as (n'&t2&σ2&Hle&Hpartial'&Hexec).
     apply bind_rep_lr_n_val in Hpartial'.
     apply exec_pool_equiv_alt_err in Hexec.
     inversion Hexec; subst; try congruence.
-    cut (@non_errorable _ _ Λ e1 σ2); eauto.
-    eapply (soundness (M:=iResUR Σ) _ (S k + S (S n'))).
+    iAssert (▷^(S k + S (S n')) ⌜@non_errorable _ _ Λ e1 σ2⌝)%I with "[Hwp]" as "Herr"; last first.
+    { iApply (laterN_le (S k+ S (S n'))); first by lia.
+      iApply laterN_mono; last by iApply "Herr". iPureIntro. eauto. }
     rewrite laterN_plus.
     iApply bupd_iter_laterN_mono; first by reflexivity.
-    iMod wsat_alloc as (Hinv) "[Hw HE]". specialize (Hwp _).
+    iMod wsat_alloc as (Hinv) "[Hw HE]". iSpecialize ("Hwp" $! _).
     iModIntro. iNext.
-    iApply (bupd_iter_mono k with "[Hw HE] []"); last by iApply Hwp.
+    iApply (bupd_iter_mono k with "[Hw HE] [Hwp]"); last by iApply "Hwp".
     iIntros "Hwp". rewrite {1}uPred_fupd_eq.
     iMod ("Hwp" with "[$Hw $HE]") as ">(Hw & HE & Hwp)".
     iDestruct "Hwp" as (Istate) "[HI Hwp]".
     iApply (@wptp_safe _ _ _ (IrisG _ _ _ Hinv Istate)); eauto with iFrame.
     set_solver+.
+Qed.
+
+Theorem wp_strong_adequacy {T} OpT Σ Λ `{invPreG Σ} s (e: proc OpT T) σ φ k:
+  (∀ `{Hinv : invG Σ},
+     Nat.iter k (λ P, |==> ▷ P)%I (|={⊤}=> ∃ stateI : State Λ → iProp Σ,
+       let _ : irisG OpT Λ Σ := IrisG _ _ _ Hinv stateI in
+       stateI σ ∗ WP e @ s; ⊤ {{ v, ∀ σ, stateI σ ={⊤,∅}=∗ ⌜ φ v σ ⌝ }})%I) →
+  adequate s e σ φ.
+Proof.
+  intros Hwp. unshelve (eapply @adequacy_int_to_ext); eauto.
+  iApply wp_strong_adequacy_internal. iIntros (Hinv). iApply Hwp.
 Qed.
 
 Theorem wp_adequacy {T} OpT Σ Λ `{invPreG Σ} s (e: proc OpT T) σ φ k:
@@ -369,50 +459,63 @@ Proof.
   }
 Qed.
 
-Inductive seq_star_exec_steps {R} {OpT} {Λ: Layer OpT} (rec: proc OpT R)
-  : Λ.(State) → Λ.(State) → nat → Prop :=
-  | sses_nil σ :
-      seq_star_exec_steps rec σ σ O
-  | sses_cons σ1 σ1' σ2 ret σ3 k n :
-      Λ.(crash_step) σ1 (Val σ1' ()) →
-      bind_rep_n n (exec_pool Λ) [existT R rec] σ1' (Val σ2 ret) →
-      seq_star_exec_steps rec σ2 σ3 k →
-      seq_star_exec_steps rec σ1 σ3 (S n + S k).
-
-Lemma seq_star_exec_steps_intro {R} {OpT} {Λ: Layer OpT} (rec: proc OpT R) σhalt σcrash:
-  seq_star (_ <- Λ.(crash_step); exec_halt Λ rec) σhalt (Val σcrash ()) →
-  ∃ k, seq_star_exec_steps rec σhalt σcrash k.
+Lemma rexec_n_iter_split {R} OpT (Λ: Layer OpT) (rec: proc OpT R) σhalt ret n2 n3:
+  (_ <- seq_star_exec_steps Λ rec n2; _ <- Λ.(crash_step); _ <- exec_n Λ rec n3; pure ())
+           σhalt ret →
+  ∃ (σcrash σrec : Λ.(State)) n2' n3',
+    (n2 + n3 >= n2' + n3')%nat ∧
+    (seq_star_exec_steps Λ rec n2') σhalt (Val σcrash ())
+    ∧ Λ.(crash_step) σcrash (Val σrec ())
+    ∧ (_ <- exec_n Λ rec n3'; pure ()) σrec ret.
 Proof.
-  intros Hstar.
-  remember (Val σcrash ()) as ret eqn:Heq; revert Heq.
-  induction Hstar as [|??? [] Hstep|]; inversion 1; subst.
-  - exists O. econstructor.
-  - destruct Hstep as ([]&σ'&Hcrash&Hexec).
-    edestruct IHHstar as (k&Hrest); auto.
-    destruct Hexec as (?&?&Hpartial&Hpure).
-    inversion Hpure; subst.
-    apply bind_star_inv_rep_n in Hpartial as (n&Hbind).
-    exists (S n + S k)%nat; econstructor; eauto.
+  intros Hrec. destruct ret as [b t|].
+  {
+    destruct Hrec as ([]&σhalt_rec&Hhd&([]&?&?&?)).
+    do 4 eexists; split_and!; eauto.
+  }
+  {
+    destruct Hrec as [Hstar_err|([]&σhalt_rec&Hhd&Hrest)].
+    - remember Err as ret eqn:Heq.
+      revert Heq; induction Hstar_err; intros; try congruence; subst.
+      * edestruct IHHstar_err as (σcrash&σrec_err&n2'&n3'&Heq&Hstar&?); auto.
+        eexists σcrash, σrec_err, _, _; split; last first.
+        { split; eauto. econstructor; eauto. }
+        { lia. }
+      * do 4 eexists; split; last first.
+        { split. econstructor. split. eauto. left; eauto. }
+        { lia. }
+    - destruct Hrest as [|([]&σ&?&?)].
+      { exfalso. eapply crash_non_err; eauto. }
+      do 4 eexists; split_and!; eauto.
+  }
 Qed.
 
-Theorem wp_recovery_nonstuck_internal {T R} OpT Σ Λ `{invPreG Σ} s (e: proc OpT T) (rec: proc OpT R)
-        σ1 φ φinv φrec :
-  (∀ `{Hinv : invG Σ},
+Definition wp_recovery {T R OpT} Σ Λ `{invPreG Σ} s (e: proc OpT T) (rec: proc OpT R)
+        σ1 φ φrec k :=
+  (Nat.iter k (λ P, |==> ▷ P)%I
+    (∃ (φinv : Λ.(State) → iProp Σ), ∀ `{Hinv : invG Σ},
      (* normal execution *)
      (|={⊤}=> ∃ stateI : State Λ → iProp Σ,
        let _ : irisG OpT Λ Σ := IrisG _ _ _ Hinv stateI in
-       stateI σ1 ∗ WP e @ s; ⊤ {{ v, ∀ σ, stateI σ ={⊤,∅}=∗ ⌜ φ v σ ⌝ }}
-       ∗ (∀ σ2', stateI σ2' ={⊤,∅}=∗ φinv σ2')
+       stateI σ1 ∗ WP e @ s; ⊤ {{ v, ∀ σ, stateI σ ={⊤,∅}=∗ φ v σ }}
+                 ∗ (∀ σ2', stateI σ2' ={⊤,∅}=∗ φinv σ2')
      ∗
      (* recovery execution *)
      □ (∀ `{Hinv : invG Σ} σ1 σ1' (Hcrash: Λ.(crash_step) σ1 (Val σ1' tt)),
-     (φinv σ1 ={⊤}=∗ ∃ stateI : State Λ → iProp Σ,
-       let _ : irisG OpT Λ Σ := IrisG _ _ _ Hinv stateI in
-       stateI σ1' ∗ WP rec @ s; ⊤ {{ _, ∀ σ, stateI σ ={⊤, ∅}=∗ ⌜ φrec σ ⌝ }}
-         ∗ (∀ σ2', stateI σ2' ={⊤,∅}=∗ φinv σ2')))))%I →
+           (φinv σ1 ={⊤}=∗ ∃ stateI : State Λ → iProp Σ,
+                         let _ : irisG OpT Λ Σ := IrisG _ _ _ Hinv stateI in
+                         stateI σ1'
+                                ∗ WP rec @ s; ⊤ {{ _, ∀ σ, stateI σ ={⊤, ∅}=∗ φrec σ }}
+                                ∗ (∀ σ2', stateI σ2' ={⊤,∅}=∗ φinv σ2'))))))%I.
+
+(*
+Theorem wp_recovery_nonstuck_internal {T R} OpT Σ Λ `{invPreG Σ} s (e: proc OpT T) (rec: proc OpT R)
+        σ1 φ φrec k :
+    wp_recovery Λ s e rec σ1 φ φrec k →
     s = NotStuck →
     ¬ Λ.(rexec) e (rec_singleton rec) σ1 Err.
 Proof.
+  Admitted.
   - rewrite /rexec/exec_recover => Hwp Hnstuck Hrexec.
     eapply rimpl_elim in Hrexec; last first.
     { setoid_rewrite exec_seq_partial_singleton.
@@ -429,9 +532,12 @@ Proof.
     clear Hrexec.
     (* Show that we couldn't have crashed during e *)
     destruct Hrexec' as [|(tp&σhalt&Hpartial&Hrec)].
-    { eapply wp_strong_adequacy with (k := O); eauto.
+    { eapply wp_strong_adequacy_internal with (k0 := k); eauto.
       intros Hinv.
-      iPoseProof (Hwp $! Hinv) as "Hwp".
+      iPoseProof Hwp as "Hwp".
+      iApply (bupd_iter_mono with "[] Hwp"). iClear "Hwp". iIntros "Hwp".
+      iDestruct "Hwp" as (φinv) "Hwp".
+      iSpecialize ("Hwp" $! Hinv).
       iMod "Hwp" as (stateI) "(Hσ&Hwp_e&?&_)".
       iExists stateI. iIntros "{$Hσ} !> "; auto.
     }
@@ -440,19 +546,23 @@ Proof.
         as (σcrash&σrec_err&Hstar&Hcrash&Herr); eauto.
 
     apply bind_star_inv_rep_n in Hpartial as (n&Hpartial).
-    apply seq_star_exec_steps_intro in Hstar as (k&Hstar).
+    apply seq_star_exec_steps_intro in Hstar as (k0&Hstar).
     apply bind_pure_no_err in Herr.
     edestruct (bind_star_inv_rep_n) as (n'&Herr'); first by eapply Herr.
 
-    edestruct (wp_strong_adequacy _ s rec σrec_err (λ _ σ2, True)
-               (S n + S k )) as (Had&?); eauto; last first.
+    edestruct (wp_strong_adequacy_internal _ s rec σrec_err (λ _ σ2, True%I)
+               (S k + S n +S k0)) as (Had&?); eauto; last first.
     { intuition. }
 
 
     intros Hinv.
     rewrite Nat_iter_add.
+    rewrite Nat_iter_add.
     iMod wsat_alloc as (Hinv') "[Hw HE]".
-    iPoseProof (Hwp $! Hinv') as "Hwp".
+    iPoseProof Hwp as "Hwp".
+    iApply (bupd_iter_mono with "[Hw HE] Hwp"). iClear "Hwp". iIntros "Hwp".
+    iDestruct "Hwp" as (φinv) "Hwp".
+    iSpecialize ("Hwp" $! Hinv').
     rewrite uPred_fupd_eq.
     iMod ("Hwp" with "[$Hw $HE]") as ">(Hw & HE & Hrest)".
     iDestruct "Hrest" as (stateI) "(Hσ&Hwp_e&Hinv&#Hwp_rec)".
@@ -468,16 +578,17 @@ Proof.
     }
     iApply (bupd_iter_mono with "[] Hσhalt"); iIntros "Hσhalt".
 
-    iClear "Hwp".
     clear Hpartial Hrec.
 
-    iAssert (Nat.iter (S k) (λ P, |==> ▷ P)%I (|==> ◇ φinv σcrash))%I with "[Hσhalt]" as "Hinv'".
+    iAssert (Nat.iter (S k0) (λ P, |==> ▷ P)%I (|==> ◇ φinv σcrash))%I with "[Hσhalt]" as "Hinv'".
     {
       clear Hcrash σrec_err Herr Herr'.
-      iInduction Hstar as [| σhalt σhalt' σmid ret σcrash k m Hcrash Hrep Hind ] "IH".
-      { iIntros "!> !>"; auto. }
+      remember (Val σcrash ()) as ret eqn:Heq.
+      iInduction Hstar as [| k0 σhalt σhalt' σmid ret ? m Hcrash Hrep Hind ] "IH".
+      { inversion Heq; subst. iIntros "!> !>"; auto. }
+      inversion Heq; subst.
 
-      rewrite (Nat_iter_S (S m + S k)).
+      rewrite (Nat_iter_S (S m + S k1)).
       rewrite Nat_iter_add.
       iMod wsat_alloc as (Hinv'') "[Hw HE]".
       iSpecialize ("Hwp_rec" $! _ _ _ Hcrash).
@@ -504,61 +615,49 @@ Proof.
     iApply wp_wand_l; iFrame.
     iIntros (?) "Hwand". iIntros. iApply @fupd_mask_weaken; auto.
 Qed.
+*)
 
-Theorem wp_recovery_adequacy {T R} OpT Σ Λ `{invPreG Σ} s (e: proc OpT T) (rec: proc OpT R)
-        σ1 φ φinv (φrec : Λ.(State) → Prop) :
-  (∀ `{Hinv : invG Σ},
-     (* normal execution *)
-     (|={⊤}=> ∃ stateI : State Λ → iProp Σ,
-       let _ : irisG OpT Λ Σ := IrisG _ _ _ Hinv stateI in
-       stateI σ1 ∗ WP e @ s; ⊤ {{ v, ∀ σ, stateI σ ={⊤,∅}=∗ ⌜ φ v σ ⌝ }}
-       ∗ (∀ σ2', stateI σ2' ={⊤,∅}=∗ φinv σ2')
-     ∗
-     (* recovery execution *)
-     □ (∀ `{Hinv : invG Σ} σ1 σ1' (Hcrash: Λ.(crash_step) σ1 (Val σ1' tt)),
-     (φinv σ1 ={⊤}=∗ ∃ stateI : State Λ → iProp Σ,
-       let _ : irisG OpT Λ Σ := IrisG _ _ _ Hinv stateI in
-       stateI σ1' ∗ WP rec @ s; ⊤ {{ _, ∀ σ, stateI σ ={⊤, ∅}=∗ ⌜ φrec σ ⌝ }}
-         ∗ (∀ σ2', stateI σ2' ={⊤,∅}=∗ φinv σ2')))))%I →
+Theorem wp_recovery_adequacy_internal {T R} OpT Σ Λ `{invPreG Σ} s (e: proc OpT T) (rec: proc OpT R)
+        σ1 φ (φrec : Λ.(State) → iProp Σ) k:
   s = NotStuck →
-  recv_adequate s e rec σ1 φ φrec.
+  wp_recovery Λ s e rec σ1 φ φrec k ⊢
+  recv_adequate_internal s e rec σ1 φ φrec k.
 Proof.
-  intros Hwp ?. split.
-  - intros σ2 ? Hexec. eapply wp_strong_adequacy with (k := 0); eauto.
-    intros Hinv.
-    iPoseProof (Hwp $! Hinv) as "Hwp".
+  iIntros (?) "Hwp". iSplit; [| iSplit].
+  - iIntros (? σ2 ? Hexec).
+    iApply (wp_strong_adequacy_internal with "[Hwp]"); last eauto.
+    iIntros (Hinv). iApply (bupd_iter_mono with "[] Hwp"). iIntros "Hwp".
+    iDestruct "Hwp" as (φinv) "Hwp".
+    iSpecialize ("Hwp" $! Hinv).
     iMod "Hwp" as (stateI) "(Hσ&Hwp_e&?&_)".
     iExists stateI. iIntros "{$Hσ} !> "; auto.
-  - rewrite /rexec/exec_recover => σ2 [] Hrexec.
-    eapply requiv_no_err_elim in Hrexec; first last.
-    { eapply wp_recovery_nonstuck_internal; eauto. }
-    { setoid_rewrite exec_seq_partial_singleton.
-      setoid_rewrite <-bind_assoc at 2.
-      setoid_rewrite <-seq_unit_sliding_equiv.
-      setoid_rewrite bind_assoc.
-      reflexivity.
-    }
-    simpl exec_seq in Hrexec.
-
+  - iIntros (n0 σ2 [] Hrexec_n). 
+    inversion Hrexec_n as [? ? n k0 n3 Heq Hrexec]; subst.
+    clear Hrexec_n.
     destruct Hrexec as (tp&σhalt&Hpartial&Hrec).
     destruct Hrec as ([]&σcrash&Hstar&Hfin).
     destruct Hfin as ([]&σcrash'&Hcrash&Hfin).
-
-
-    apply bind_star_inv_rep_n in Hpartial as (n&Hpartial).
-    apply seq_star_exec_steps_intro in Hstar as (k&Hstar).
     destruct Hfin as (?&?&Hexec&Hp).
     inversion Hp; subst. clear Hp.
 
-    edestruct (wp_strong_adequacy _ NotStuck rec σcrash' (λ _ s, φrec s)
-               (S n + S k )) as (Had&?); eauto; last first.
-    { edestruct Had; intuition eauto. }
+    iPoseProof (wp_strong_adequacy_internal _ NotStuck rec σcrash' (λ _ s, φrec s)
+                                        (S k + S n + S k0 ) with "[Hwp]") as "(Had&_)"; last first.
+    {
+      assert ((S k + (5 + (n + k0 + n3))) = (S (S k + S n + S k0) + S (S n3)))%nat as Heq.
+      { lia. }
+      iApply bupd_iter_mono; last first.
+      { rewrite Heq. iApply "Had". eauto. }
+      iIntros "H". iDestruct "H" as (? ?) "$".
+    }
 
 
-    intros Hinv.
+    iIntros (Hinv).
+    rewrite Nat_iter_add.
     rewrite Nat_iter_add.
     iMod wsat_alloc as (Hinv') "[Hw HE]".
-    iPoseProof (Hwp $! Hinv') as "Hwp".
+    iApply (bupd_iter_mono with "[Hw HE] Hwp"). iIntros "Hwp".
+    iDestruct "Hwp" as (φinv) "Hwp".
+    iSpecialize ("Hwp" $! Hinv').
     rewrite uPred_fupd_eq.
     iMod ("Hwp" with "[$Hw $HE]") as ">(Hw & HE & Hrest)".
     iDestruct "Hrest" as (stateI) "(Hσ&Hwp_e&Hinv&#Hwp_rec)".
@@ -574,16 +673,17 @@ Proof.
     }
     iApply (bupd_iter_mono with "[] Hσhalt"); iIntros "Hσhalt".
 
-    iClear "Hwp".
     clear Hpartial.
 
-    iAssert (Nat.iter (S k) (λ P, |==> ▷ P)%I (|==> ◇ φinv σcrash))%I with "[Hσhalt]" as "Hinv'".
+    iAssert (Nat.iter (S k0) (λ P, |==> ▷ P)%I (|==> ◇ φinv σcrash))%I with "[Hσhalt]" as "Hinv'".
     {
       clear Hcrash Hexec σcrash' σ2 x Hexec.
-      iInduction Hstar as [| σhalt σhalt' σmid ret σcrash k m Hcrash Hrep Hind ] "IH".
-      { iIntros "!> !>"; auto. }
+      remember (Val σcrash ()) as ret eqn:Heq.
+      iInduction Hstar as [| k0 σhalt σhalt' σmid ret ? m Hcrash Hrep Hind|] "IH"; last by congruence.
+      { inversion Heq; subst. iIntros "!> !>"; auto. }
+      inversion Heq; subst.
 
-      rewrite (Nat_iter_S (S m + S k)).
+      rewrite (Nat_iter_S (S m + S k1)).
       rewrite Nat_iter_add.
       iMod wsat_alloc as (Hinv'') "[Hw HE]".
       iSpecialize ("Hwp_rec" $! Hinv'').
@@ -608,9 +708,103 @@ Proof.
     iSpecialize ("Hwp_rec" $! Hinv σcrash σcrash' Hcrash with "Hinv'").
     iMod "Hwp_rec" as (stateI'') "[Hσ [H _]]"; eauto.
     iExists stateI''. iIntros "{$Hσ} !> "; auto.
-  - eapply wp_recovery_nonstuck_internal; eauto.
+
+  - iIntros (n _ Hrexec_n). 
+    inversion Hrexec_n as [?? n1 n2 n3 Heq Hrexec_n']; subst.
+    destruct Hrexec_n' as [|(tp&σhalt&Hpartial&Hrec)].
+    {
+      iApply laterN_le; last first.
+      { iApply (wp_strong_adequacy_internal with "[Hwp]"); eauto.
+        iIntros (Hinv).
+        iApply (bupd_iter_mono with "[] Hwp"). iIntros "Hwp".
+        iDestruct "Hwp" as (φinv) "Hwp".
+        iSpecialize ("Hwp" $! Hinv).
+        iMod "Hwp" as (stateI) "(Hσ&Hwp_e&?&_)".
+        iExists stateI. iIntros "{$Hσ} !> "; auto.
+      }
+      { lia. }
+    }
+    edestruct (@rexec_n_iter_split)
+        as (σcrash&σrec_err&k0&n'&Hle&Hstar&Hcrash&Herr); eauto.
+    apply bind_pure_no_err in Herr.
+
+    iPoseProof (wp_strong_adequacy_internal _ NotStuck rec σrec_err (λ _ s, φrec s)
+                                        (S k + S n1 + S k0) with "[Hwp]") as "(_&Hnst)"; last first.
+    { iApply laterN_le; last iApply "Hnst"; eauto.
+      lia.
+    }
+
+    iIntros (Hinv).
+    rewrite Nat_iter_add.
+    rewrite Nat_iter_add.
+    iMod wsat_alloc as (Hinv') "[Hw HE]".
+    iApply (bupd_iter_mono with "[Hw HE] Hwp"). iIntros "Hwp".
+    iDestruct "Hwp" as (φinv) "Hwp".
+    iSpecialize ("Hwp" $! Hinv').
+    rewrite uPred_fupd_eq.
+    iMod ("Hwp" with "[$Hw $HE]") as ">(Hw & HE & Hrest)".
+    iDestruct "Hrest" as (stateI) "(Hσ&Hwp_e&Hinv&#Hwp_rec)".
+    iAssert (Nat.iter (S n1) (λ P, |==> ▷ P)%I (|==> ◇ φinv σhalt))%I with "[Hw HE Hσ Hwp_e Hinv]"
+      as "Hσhalt".
+    {
+      iDestruct (wptp_steps_state_inv with "[-Hinv]") as "H".
+      { eapply Hpartial. }
+      { iFrame. done. }
+      iApply (bupd_iter_mono with "[Hinv] H").
+      iIntros "(Hw&HE&Hstate)". iSpecialize ("Hinv" with "Hstate").
+      iMod ("Hinv" with "[$Hw $HE]") as "(?&?&$)"; auto.
+    }
+    iApply (bupd_iter_mono with "[] Hσhalt"); iIntros "Hσhalt".
+
+    clear Hpartial Hrec.
+
+    iAssert (Nat.iter (S k0) (λ P, |==> ▷ P)%I (|==> ◇ φinv σcrash))%I with "[Hσhalt]" as "Hinv'".
+    {
+      clear Hcrash σrec_err Herr.
+      remember (Val σcrash ()) as ret eqn:Heq.
+      iInduction Hstar as [| k0 σhalt σhalt' σmid ret ? m Hcrash Hrep Hind|] "IH"; last by congruence.
+      { inversion Heq; subst. iIntros "!> !>"; auto. }
+      inversion Heq; subst.
+
+      rewrite (Nat_iter_S (S m + S k1)).
+      rewrite Nat_iter_add.
+      iMod wsat_alloc as (Hinv'') "[Hw HE]".
+      iSpecialize ("Hwp_rec" $! _ _ _ Hcrash).
+      rewrite uPred_fupd_eq.
+      iMod "Hσhalt". iModIntro. iMod "Hσhalt". iNext.
+      iMod ("Hwp_rec" with "Hσhalt [$Hw $HE]") as ">(Hw & HE & Hrest)".
+      iDestruct "Hrest" as (stateI') "(Hs&Hwp&Hinv)".
+      iDestruct (wptp_steps_state_inv with "[-Hinv]") as "H".
+      { eapply Hrep. }
+      { iFrame. done. }
+      iApply (bupd_iter_mono with "[Hinv] H").
+      iIntros "(Hw&HE&Hstate)".
+      iApply "IH"; auto.
+      { iPureIntro. lia. }
+      iSpecialize ("Hinv" with "[Hstate]"); eauto.
+      rewrite /uPred_fupd_def.
+      by iMod ("Hinv" with "[$Hw $HE]") as ">(?&?&$)".
+    }
+
+
+    iApply (bupd_iter_mono with "[] Hinv'"); iIntros ">>Hinv'".
+    iSpecialize ("Hwp_rec" $! Hinv σcrash σrec_err Hcrash with "Hinv'").
+    iMod "Hwp_rec" as (stateI'') "[Hσ [H _]]"; eauto.
+    iExists stateI''. iIntros "{$Hσ} !> "; auto.
 Qed.
 
+Theorem wp_recovery_adequacy {T R} OpT Σ Λ `{invPreG Σ} s (e: proc OpT T) (rec: proc OpT R)
+        σ1 φ (φrec : Λ.(State) → Prop) k:
+  s = NotStuck →
+  wp_recovery Λ s e rec σ1 (fun v σ => ⌜ φ v σ ⌝)%I (fun σ => ⌜ φrec σ ⌝)%I k →
+  recv_adequate s e rec σ1 φ φrec.
+Proof.
+  intros ? Hwp. subst. unshelve (eapply @recv_adequacy_int_to_ext); eauto.
+  iApply wp_recovery_adequacy_internal; eauto.  iApply Hwp.
+Qed.
+
+(* FIXME: add outer iter of k *)
+(*
 Theorem wp_recovery_invariance {T R} OpT Σ Λ `{invPreG Σ} s (e: proc OpT T) (rec: proc OpT R)
         σ1 φ φrec φinv ρ :
   (∀ `{Hinv : invG Σ},
@@ -633,7 +827,8 @@ Proof.
   intros Hwp ?.
   assert (recv_adequate s e rec σ1 φ φrec).
   {
-    eapply wp_recovery_adequacy with (φinv0 := φinv); first eauto.
+    eapply recv_adequacy_int_to_ext.
+    eapply wp_recovery_adequacy_internal with (φinv0 := φinv); first eauto.
     - intros. iIntros. iPoseProof (Hwp $! Hinv) as "Hwp".
       iMod "Hwp" as (stateI) "(Hσ&Hwp_e&Hφ&#Hwp_rec)".
       iModIntro. iExists stateI. iFrame.
@@ -724,3 +919,119 @@ Proof.
   - iApply wp_wand_l; iFrame. iIntros; auto.
   - iIntros. iMod ("Hinv" with "[$]") as "(?&$)"; auto.
 Qed.
+*)
+
+Fixpoint wp_proc_seq {T R} OpT Σ Λ `{invPreG Σ} s (es: proc_seq OpT T) (rec: proc OpT R)
+        σ1 φ (φrec : Λ.(State) → iProp Σ) : iProp Σ :=
+  match es with
+  | Proc_Seq_Final e => wp_recovery Λ s e rec σ1 φ φrec O
+  | @Proc_Seq_Bind _ _ T0 e es' =>
+    wp_recovery Λ s e rec σ1
+                (λ v σ2, wp_proc_seq Λ s (es' (Normal (existT T0 v))) rec σ2 φ φrec)
+                (λ σ2, wp_proc_seq Λ s (es' (Recovered (existT _ tt))) rec σ2 φ φrec)
+                O
+  end.
+
+(* TODO: there is a lot of silly case splitting because of how these 
+   lemmas are structured *)
+(*
+Theorem wp_proc_seq_adequacy {T R} OpT Σ Λ `{invPreG Σ} s (es: proc_seq OpT T) (rec: proc OpT R)
+        σ1 φ φrec k:
+  Nat.iter k (λ P, |==> ▷ P)%I
+             (wp_proc_seq Λ s es rec σ1 (λ v σ2, ⌜ φ v σ2 ⌝%I) (λ σ2, ⌜ φrec σ2 ⌝%I)) →
+  s = NotStuck →
+  proc_seq_adequate s es rec σ1 φ φrec.
+Proof.
+  intros Hwp ->.
+  split.
+  - revert k σ1 Hwp. induction es => k σ1 Hwp σ2 res.
+    * destruct 1 as [Hnorm|Hrecv].
+      ** destruct Hnorm as (v&?&Hexec&Hpure). inversion Hpure; subst.
+         eapply recv_adequate_normal_result with (s := NotStuck); eauto.
+         unshelve (eapply recv_adequacy_int_to_ext); eauto.
+         unshelve (iApply wp_recovery_adequacy_internal); eauto.
+         iApply Hwp.
+      ** destruct Hrecv as (v&?&Hrexec&Hpure). inversion Hpure; subst.
+         eapply recv_adequate_result with (s := NotStuck); eauto.
+         unshelve (eapply recv_adequacy_int_to_ext); eauto.
+         unshelve (iApply wp_recovery_adequacy_internal); eauto.
+         iApply Hwp.
+    * destruct 1 as (res0&σ1'&Hhd&Hrest).
+      destruct Hhd as [Hnorm|Hrecv].
+      ** destruct Hnorm as (v&?&Hexec&Hpure). inversion Hpure; subst.
+         eapply exec_equiv_exec_n in Hexec as (n&Hexec).
+         iPoseProof Hwp as "Hwp".
+         eapply H0; eauto.
+         eapply wp_recovery_adequacy_internal in Hwp; auto.
+         eapply recv_adequate_internal_normal_result in Hwp; eauto.
+         eapply H0; eauto.
+         iApply (bupd_iter_mono); last iApply Hwp.
+         iIntros "Hrec". iDestruct "Hrec" as (v' Hp) "Hrec".
+         subst. iApply "Hrec".
+      ** destruct Hrecv as ([]&?&Hrexec&Hpure). inversion Hpure; subst.
+         eapply wp_recovery_adequacy_internal in Hwp; auto.
+         eapply rexec_equiv_rexec_n' in Hrexec as (n&Hexec).
+         { eapply recv_adequate_internal_result in Hwp as Hwp; eauto.
+           eapply H0; eauto. }
+         { eapply recv_adequate_internal_not_stuck in Hwp as Hwp; eauto. }
+  - revert k σ1 Hwp. induction es => k σ1 Hwp _.
+    * destruct 1 as [Hnorm%bind_pure_no_err|Hrecv%bind_pure_no_err].
+      ** eapply exec_err_rexec_err in Hnorm.
+         eapply recv_adequate_internal_not_stuck; eauto.
+         eapply wp_recovery_adequacy_internal; eauto.
+      ** eapply recv_adequate_internal_not_stuck; eauto.
+         eapply wp_recovery_adequacy_internal; eauto.
+    * destruct 1 as [[Hnorm%bind_pure_no_err|Hrec%bind_pure_no_err]|Htl].
+      ** eapply exec_err_rexec_err in Hnorm.
+         eapply recv_adequate_internal_not_stuck; eauto.
+         eapply wp_recovery_adequacy_internal; eauto.
+      ** eapply recv_adequate_internal_not_stuck; eauto.
+         eapply wp_recovery_adequacy_internal; eauto.
+      ** destruct Htl as (?&σ1'&[Hnorm|Hrec]&?).
+         *** destruct Hnorm as (v&?&Hexec&Hpure). inversion Hpure; subst.
+             eapply wp_recovery_adequacy_internal in Hwp; auto.
+             eapply exec_equiv_exec_n in Hexec as (n&Hexec).
+             eapply recv_adequate_internal_normal_result in Hwp; eauto.
+             eapply H0; eauto.
+             iApply (bupd_iter_mono); last iApply Hwp.
+             iIntros "Hrec". iDestruct "Hrec" as (v' Hp) "Hrec".
+             subst. iApply "Hrec".
+         *** destruct Hrec as ([]&?&Hexec&Hpure). inversion Hpure; subst.
+             eapply wp_recovery_adequacy_internal in Hwp; auto.
+             eapply rexec_equiv_rexec_n' in Hexec as (n&Hexec).
+             { eapply recv_adequate_internal_result in Hwp as Hwp; eauto.
+               eapply H0; eauto. }
+             { eapply recv_adequate_internal_not_stuck in Hwp as Hwp; eauto. }
+Qed.
+*)
+
+(*
+Theorem wp_proc_seq_adequacy' {T R} OpT Σ Λ `{invPreG Σ} s (es: proc_seq OpT T) (rec: proc OpT R)
+        σ1 φ φrec k:
+  Nat.iter k (λ P, |==> ▷ P)%I
+             (wp_proc_seq Λ s es rec σ1 (λ v σ2, ⌜ φ v σ2 ⌝%I) (λ σ2, ⌜ φrec σ2 ⌝%I)) →
+  s = NotStuck →
+  proc_seq_adequate s es rec σ1 φ φrec.
+Proof.
+  intros Hwp ->.
+  revert k σ1 Hwp. induction es => k σ1 Hwp.
+  - split. 
+    * destruct 1 as [Hnorm|Hrecv].
+      ** destruct Hnorm as (v&?&Hexec&Hpure). inversion Hpure; subst.
+         eapply recv_adequate_normal_result; eauto.
+         eapply recv_adequacy_int_to_ext.
+         eapply wp_recovery_adequacy_internal; eauto.
+      ** destruct Hrecv as (v&?&Hrexec&Hpure). inversion Hpure; subst.
+         eapply recv_adequate_result; eauto.
+         eapply recv_adequacy_int_to_ext.
+         eapply wp_recovery_adequacy_internal; eauto.
+    * intros ?. destruct 1 as [Hnorm%bind_pure_no_err|Hrecv%bind_pure_no_err].
+      ** eapply exec_err_rexec_err in Hnorm.
+         eapply recv_adequate_internal_not_stuck; eauto.
+         eapply wp_recovery_adequacy_internal; eauto.
+      ** eapply recv_adequate_internal_not_stuck; eauto.
+         eapply wp_recovery_adequacy_internal; eauto.
+  - split. intros.
+    * destruct H1 as (res0&σ1'&Hhd&Hrest).
+      destruct Hhd.
+*)
