src/CSL/RefinementAdequacy.v
@@ -12,42 +12,264 @@ From iris.proofmode Require Import tactics.
 Unset Implicit Arguments.
 
 Import RelationNotations.
-Definition pool_map_incl {OpT} (tp1: gmap nat (@procT OpT)) (tp2: thread_pool OpT) :=
-  ∀ j e, tp1 !! j = Some e → tp2 !! j = Some e.
-
-Lemma pool_map_incl_alt {OpT} tp1 (tp2: thread_pool OpT) :
-  pool_map_incl tp1 tp2 ↔ tp1 ⊆ tpool_to_map tp2.
-Proof.
-  split.
-  - intros Hincl j.
-    rewrite /option_relation.
-    specialize (Hincl j). destruct (tp1 !! j) as [p|].
-    * rewrite (proj2 (tpool_to_map_lookup tp2 j p)); eauto.
-    * destruct (tpool_to_map tp2 !! j); eauto.
-  - intros Hincl j e Hin.
-    apply tpool_to_map_lookup.
-    specialize (Hincl j). rewrite Hin //= in Hincl.
-    destruct (tpool_to_map tp2 !! j); eauto; [ congruence | contradiction ].
-Qed.
-
 Require Import Helpers.RelationAlgebra.
-Theorem wp_recovery_crash_refinement {T R} OpTa OpTc Σ (Λa: Layer OpTa) (Λc: Layer OpTc)
+
+Definition wp_recovery_refinement {T R OpTa OpTc} Σ (Λa: Layer OpTa) (Λc: Layer OpTc)
         `{invPreG Σ} `{cfgPreG OpTa Λa Σ}
-        (ea: proc OpTa T) (ec: proc OpTc T) (rec: proc OpTc R)
-        (φinv : forall {_ : @cfgG OpTa Λa Σ}, Λc.(State) → iProp Σ)
-        (absr: relation Λa.(State) Λc.(State) unit) E
-        (Habsr_no_err: ∀ σa, ¬ absr σa Err):
-  nclose sourceN ⊆ E →
-  (∀ (σ1a: Λa.(State)) σ1c,
-      absr σ1a (Val σ1c tt) →
-      (∀ `{Hinv : invG Σ} `{Hcfg: cfgG OpTa Λa Σ},
+        (ea: proc OpTa T) (ec: proc OpTc T) (rec: proc OpTc R) σ1a σ1c φ φrec E k :=
+  Nat.iter k (λ P, |==> ▷ P)%I
+    ((⌜ nclose sourceN ⊆ E ⌝ ∧
+             ∃ (φinv : forall {_ : @cfgG OpTa Λa Σ}, Λc.(State) → iProp Σ),
+         ∀ `{Hinv : invG Σ} `{Hcfg: cfgG OpTa Λa Σ},
           (|={⊤}=> ∃ stateI : State Λc → iProp Σ,
              let _ : irisG OpTc Λc Σ := IrisG _ _ _ Hinv stateI in
              (source_ctx ([existT _ ea], σ1a) ∗ O ⤇ ea ∗ source_state σ1a)
                ={⊤}=∗
                stateI σ1c
                ∗ WP ec @ NotStuck; ⊤ {{ v, O ⤇ of_val v
-                    ∗ (∀ σ2c, stateI σ2c ={⊤,E}=∗ ∃ σ2a, source_state σ2a ∗ ⌜absr σ2a (Val σ2c tt)⌝)}}
+                    ∗ (∀ σ2c, stateI σ2c ={⊤,E}=∗ ∃ σ2a, source_state σ2a ∗ φ v σ2a σ2c)}}
+                    ∗ (∀ σ2c, stateI σ2c ={⊤,E}=∗ φinv σ2c)
+        ∗
+        □ (∀ `{Hinv : invG Σ} `{Hcfg: cfgG OpTa Λa Σ} σ1c σ1c'
+           (Hcrash: Λc.(crash_step) σ1c (Val σ1c' tt)),
+            (φinv σ1c ={⊤}=∗ ∃ stateI : State Λc → iProp Σ,
+               let _ : irisG OpTc Λc Σ := IrisG _ _ _ Hinv stateI in
+               stateI σ1c'
+               ∗ WP rec @ NotStuck; ⊤ {{ v, (∀ σ2c, stateI σ2c ={⊤,E}=∗
+                   ∃ σ2a σ2a', source_state σ2a ∗ ⌜Λa.(crash_step) σ2a (Val σ2a' tt) ⌝ ∗
+                               φrec σ2a' σ2c )}}
+               ∗ (∀ σ2c, stateI σ2c ={⊤,E}=∗ φinv σ2c))))))%I.
+
+Fixpoint map_proc_seq {OpTa OpTc T} (f: ∀ T, proc OpTa T → proc OpTc T) (es: proc_seq OpTa T) :=
+  match es with
+  | Proc_Seq_Final e => Proc_Seq_Final (f _ e)
+  | @Proc_Seq_Bind _ _ _  e es' =>
+    Proc_Seq_Bind (f _ e) (fun x => map_proc_seq f (es' x))
+  end.
+
+Fixpoint wp_proc_seq_refinement {T R OpTa OpTc} {Σ} (Λa: Layer OpTa) (Λc: Layer OpTc)
+        `{invPreG Σ} `{cfgPreG OpTa Λa Σ}
+        (es: proc_seq OpTa T) (rec: proc OpTc R) (f: ∀ T, proc OpTa T → proc OpTc T)
+        σ1a σ1c φ φrec E : iProp Σ :=
+  match es with
+  | Proc_Seq_Final e => wp_recovery_refinement Σ Λa Λc e (f _ e) rec σ1a σ1c φ φrec E O
+  | @Proc_Seq_Bind _ _ T0 e es' =>
+    wp_recovery_refinement Σ Λa Λc e (f _ e) rec σ1a σ1c
+      (λ v σ2a σ2c, wp_proc_seq_refinement Λa Λc (es' (Normal (existT T0 v)))
+                                           rec f σ2a σ2c φ φrec E)%I
+      (λ σ2a σ2c, wp_proc_seq_refinement Λa Λc (es' (Recovered (existT _ tt)))
+                                         rec f σ2a σ2c φ φrec E) E O
+  end.
+
+Theorem wp_recovery_refinement_adequacy_internal {T R} OpTa OpTc Σ (Λa: Layer OpTa) (Λc: Layer OpTc)
+        `{invPreG Σ} `{cfgPreG OpTa Λa Σ}
+        (ea: proc OpTa T) (ec: proc OpTc T) (rec: proc OpTc R) σ1a σ1c φ φrec E k
+        (Hno_fault : ¬ exec Λa ea σ1a Err):
+  wp_recovery_refinement Σ Λa Λc ea ec rec σ1a σ1c φ φrec E k ⊢
+  recv_adequate_internal NotStuck ec rec σ1c
+    (λ v σ2c, ∃ σ2a, ⌜ exec Λa ea σ1a (Val σ2a (existT _ v)) ⌝ ∗ φ v σ2a σ2c)%I
+    (λ σ2c, ∃ tp2 σ2a σ2a', ⌜ exec_partial Λa ea σ1a (Val σ2a tp2) ∧
+                            crash_step Λa σ2a (Val σ2a' tt) ⌝ ∗ φrec σ2a' σ2c)%I k.
+Proof.
+  iIntros "Hwp".
+  unshelve (iApply wp_recovery_adequacy_internal); eauto.
+  iApply (bupd_iter_mono with "[] Hwp"). iIntros "Hwp".
+  iDestruct "Hwp" as (Hclosure φinv) "Hwp".
+  iExists (fun σ => (∃ _ : cfgG Σ, φinv _ σ ∗ source_inv [existT T ea] σ1a)%I).
+  iIntros (Hinv).
+  assert (Inhabited Λa.(State)).
+  { eexists; eauto. }
+  iMod (source_cfg_init [existT _ ea] σ1a) as (cfgG) "(#Hsrc&Hpool&HstateA)"; auto.
+  { intros Herr; apply Hno_fault. apply exec_partial_err_exec_err; eauto. }
+  iMod ("Hwp" $! _ _) as (stateI) "Hwand".
+  iMod ("Hwand" with "[Hpool HstateA]") as "[Hstate [H [Hinv #Hφ]]]"; eauto.
+  { iFrame. iFrame "#".
+    rewrite /source_pool_map/tpool_to_map fmap_insert fmap_empty insert_empty //=.
+  }
+  iExists stateI. iIntros "{$Hstate} !>".
+  iSplitL "H"; last iSplitL "Hinv".
+  * iApply wp_wand_l; iFrame "H". iIntros (v') "[Hmapsto Hopen]".
+    iIntros (σ2c') "Hstate".
+    iMod ("Hopen" with "Hstate") as (σ2a) "(Hstate&Habsr)".
+    iInv "Hsrc" as (tp' σ') ">[Hauth Hp]" "_".
+    iDestruct "Hp" as %Hp. destruct Hp as (Hp&Hno_fault'). rewrite //= in Hp.
+    iDestruct (source_state_reconcile with "Hstate Hauth") as %Hstate; subst.
+    iDestruct (source_thread_reconcile with "Hmapsto Hauth") as %Hlookup; subst.
+    apply take_drop_middle in Hlookup.
+
+    iApply fupd_mask_weaken; first by set_solver+.
+    iExists σ'. iSplit; auto. iPureIntro. 
+    rewrite -Hlookup //= /of_val in Hp.
+    eapply exec_partial_finish; eauto.
+  * iIntros. iMod ("Hinv" with "[$]").
+    iMod (inv_open_timeless with "Hsrc") as "(?&_)"; first by eassumption.
+    iApply fupd_mask_weaken; auto.
+    { set_solver+. }
+    iFrame. iExists _; iFrame.
+  * iModIntro. iIntros (????) "Hinv".
+    iDestruct "Hinv" as (cfgG') "(?&HcfgInv)".
+    iClear "Hsrc".
+    iMod ("Hφ" with "[//] [$]") as (stateI') "(Hstate&Hwp&Hinv)".
+    iMod (inv_alloc sourceN ⊤ (source_inv _ _) with "HcfgInv") as "#cfgInv".
+    iModIntro. iExists stateI'. iFrame.
+    iSplitL "Hwp".
+    ** iApply wp_wand_l; iFrame.
+       iIntros (_) "H1".
+       iIntros (σ) "Hstate".
+       iMod ("H1" with "[$]") as (σ2a σ3a) "(Hstate&Hp&Habsr)".
+       iDestruct "Hp" as %Hcrash.
+       iMod (inv_open_timeless with "cfgInv") as "(Hinv&_)"; first by eassumption.
+       iApply fupd_mask_weaken; auto.
+       { set_solver+. }
+       iDestruct "Hinv" as (tp' σ3a') "(Hauth&%&%)".
+       iDestruct (source_state_reconcile with "Hstate Hauth") as %Hstate; subst.
+       iExists _, _, _. iFrame. iPureIntro; intuition eauto.
+    ** iIntros. iMod ("Hinv" with "[$]").
+       iMod (inv_open_timeless with "cfgInv") as "(?&_)"; first by eassumption.
+       iApply fupd_mask_weaken; auto.
+       { set_solver+. }
+       iFrame. iExists _; iFrame.
+Qed.
+
+Theorem wp_proc_seq_refinement_adequacy_internal {T R} OpTa OpTc Σ (Λa: Layer OpTa) (Λc: Layer OpTc)
+        `{invPreG Σ} `{cfgPreG OpTa Λa Σ}
+        (es: proc_seq OpTa T) (rec: proc OpTc R) f σ1c σ1a φ φrec E k
+        (Hno_fault : ¬ Λa.(proc_exec_seq) es (rec_singleton (Ret tt)) σ1a Err):
+  Nat.iter k (λ P, |==> ▷ P)%I (wp_proc_seq_refinement Λa Λc es rec f σ1a σ1c φ φrec E) ⊢
+  (∀ n σ2c res, ⌜Λc.(proc_exec_seq_n) (map_proc_seq f es) rec n σ1c (Val σ2c res)⌝ →
+                (Nat.iter (S k + n) (λ P, |==> ▷ P)%I
+                          (⌜ ∃ σ2a, Λa.(proc_exec_seq) es (rec_singleton (Ret tt))
+                                                       σ1a (Val σ2a res) ⌝ : iProp Σ))%I).
+Proof.
+  iIntros "Hwp". iIntros (n σ2c res Hexec). iRevert "Hwp".
+  iInduction es as [] "IH" forall (k n σ1c σ1a Hno_fault Hexec); iIntros "Hwp".
+  - destruct Hexec as (n1&?&Hexec). subst. destruct Hexec as [Hnorm|Hrecv].
+      ** destruct Hnorm as (v&?&Hexec&Hpure). inversion Hpure; subst.
+         unshelve (iPoseProof (wp_recovery_refinement_adequacy_internal with "Hwp") as "Hwp"); eauto.
+         { intros Hexec'. apply Hno_fault. by do 2 left. }
+         iDestruct "Hwp" as "(Hwp&_)".
+         iApply (@bupd_iter_le _ (S k + (S (S n1)))%nat); first by lia.
+         iApply bupd_iter_mono; last by iApply "Hwp".
+         iIntros "H".
+         iDestruct "H" as (v' Hp) "H". subst.
+         iDestruct "H" as (σ2a Hexeca) "H".
+         iPureIntro. eexists. left. do 2 eexists. intuition eauto. econstructor.
+      ** destruct Hrecv as ([]&?&Hrexec&Hpure). inversion Hpure; subst.
+         unshelve (iPoseProof (wp_recovery_refinement_adequacy_internal with "Hwp") as "Hwp"); eauto.
+         { intros Hexec'. apply Hno_fault. by do 2 left. }
+         iDestruct "Hwp" as "(_&(Hwp&_))".
+         iApply (@bupd_iter_le _ (S k + ((5 + n1)))%nat); first by lia.
+         iApply bupd_iter_mono; last by iApply "Hwp".
+         iIntros "H".
+         iDestruct "H" as (tp σ2a) "H". subst.
+         iDestruct "H" as (σ2a' Hexeca) "H".
+         iPureIntro. exists σ2a'.  right.
+         exists tt, σ2a'; split; last econstructor.
+         eapply rexec_singleton_ret_intro; intuition eauto.
+  - destruct Hexec as (n1&n2&Heq&(res0&σ1'&Hhd&Hrest)).
+      destruct Hhd as [Hnorm|Hrecv].
+      ** destruct Hnorm as (v&?&Hexec&Hpure). inversion Hpure; subst.
+         replace ((S k + (5 + n1 + S n2)))%nat with ((S k + 5 + n1) + S n2)%nat by lia.
+         rewrite /wp_proc_seq_refinement -/wp_proc_seq_refinement.
+         rewrite Nat_iter_add.
+         unshelve (iPoseProof (wp_recovery_refinement_adequacy_internal with "Hwp") as "Hwp"); eauto.
+         { intros Herr. apply Hno_fault. do 3 left. eauto. }
+         iDestruct "Hwp" as "(Hwp&_)".
+         iApply (@bupd_iter_le _ (S k + (S (S n1)))%nat); first by lia.
+         iApply bupd_iter_mono; last by iApply "Hwp".
+
+         iIntros "H".
+         iDestruct "H" as (v' Hp) "H". subst.
+         iDestruct "H" as (σ2a Hexeca) "H".
+         replace (S n2) with (1 + n2)%nat by auto.
+         iMod ("IH" $! _ O n2 with "[] [] H") as "H".
+         { iPureIntro. intros Herr.
+           eapply Hno_fault. right.
+           do 2 eexists; split; eauto.
+           left.
+           do 2 eexists; split; eauto.
+           econstructor.
+         }
+         { eauto. }
+         iModIntro.
+         iNext.
+         iApply bupd_iter_mono; last by iApply "H".
+         iIntros "H".
+         iDestruct "H" as (σ2a') "%".
+         iPureIntro. exists σ2a'.
+         do 2 eexists; split; eauto.
+         left. do 2 eexists; split; eauto. econstructor.
+      ** destruct Hrecv as ([]&?&Hexec&Hpure). inversion Hpure; subst.
+         replace ((S k + (5 + n1 + S n2)))%nat with ((S k + (5 + n1)) + S n2)%nat by lia.
+         rewrite /wp_proc_seq_refinement -/wp_proc_seq_refinement.
+         rewrite Nat_iter_add.
+         unshelve (iPoseProof (wp_recovery_refinement_adequacy_internal with "Hwp") as "Hwp"); eauto.
+         { intros Herr. apply Hno_fault. do 3 left. eauto. }
+         iDestruct "Hwp" as "(_&Hwp&_)".
+         iApply bupd_iter_mono; last by iApply "Hwp".
+
+         iIntros "H".
+         iDestruct "H" as (v' Hp) "H". subst.
+         iDestruct "H" as (σ2a Hexeca) "H".
+         replace (S n2) with (1 + n2)%nat by auto.
+         iMod ("IH" $! _ O n2 with "[] [] H") as "H".
+         { iPureIntro. intros Herr.
+           eapply Hno_fault. right.
+           do 2 eexists; split; eauto.
+           right.
+           do 2 eexists; split; eauto; last econstructor.
+           eapply rexec_singleton_ret_intro; intuition eauto.
+         }
+         { eauto. }
+         iModIntro.
+         iNext.
+         iApply bupd_iter_mono; last by iApply "H".
+         iIntros "H".
+         iDestruct "H" as (σ2a') "%".
+         iPureIntro. exists σ2a'.
+         do 2 eexists; split; eauto.
+         right.
+         econstructor; last econstructor.
+         econstructor; last econstructor.
+         eapply rexec_singleton_ret_intro; intuition eauto.
+Qed.
+
+Import uPred.
+Theorem wp_proc_seq_refinement_adequacy {T R} OpTa OpTc Σ (Λa: Layer OpTa) (Λc: Layer OpTc)
+        `{invPreG Σ} `{cfgPreG OpTa Λa Σ}
+        (es: proc_seq OpTa T) (rec: proc OpTc R) f σ1c σ1a φ φrec E
+        (Hno_fault : ¬ Λa.(proc_exec_seq) es (rec_singleton (Ret tt)) σ1a Err):
+  wp_proc_seq_refinement Λa Λc es rec f σ1a σ1c φ φrec E →
+  ∀ σ2c res, Λc.(proc_exec_seq) (map_proc_seq f es) (rec_singleton rec) σ1c (Val σ2c res) →
+  ∃ σ2a, Λa.(proc_exec_seq) es (rec_singleton (Ret tt)) σ1a (Val σ2a res).
+Proof.
+  intros Hwp ?? Hexec.
+  eapply proc_exec_seq_equiv_proc_exec_seq_n in Hexec as (n&?); last first.
+  { admit. (* just need to show non-error *) }
+  { eauto using crash_non_err. }
+  eapply (soundness (M:=iResUR Σ) _ (S O + n)).
+  iApply bupd_iter_laterN_mono; first by reflexivity; eauto.
+  iApply (wp_proc_seq_refinement_adequacy_internal); eauto.
+  iApply Hwp; eauto.
+Admitted.
+
+(*
+Theorem wp_recovery_crash_refinement {T R} OpTa OpTc Σ (Λa: Layer OpTa) (Λc: Layer OpTc)
+        `{invPreG Σ} `{cfgPreG OpTa Λa Σ}
+        (ea: proc OpTa T) (ec: proc OpTc T) (rec: proc OpTc R)
+        (φinv : forall {_ : @cfgG OpTa Λa Σ}, Λc.(State) → iProp Σ)
+        (absr: forall _ : @cfgG OpTa Λa Σ, Λa.(State) → Λc.(State) → iProp Σ) E:
+  nclose sourceN ⊆ E →
+  (∀ (σ1a: Λa.(State)) σ1c,
+      (∀ `{Hinv : invG Σ} `{Hcfg: cfgG OpTa Λa Σ},
+          (absr _ σ1a σ1c) -∗
+          (|={⊤}=> ∃ stateI : State Λc → iProp Σ,
+             let _ : irisG OpTc Λc Σ := IrisG _ _ _ Hinv stateI in
+             (source_ctx ([existT _ ea], σ1a) ∗ O ⤇ ea ∗ source_state σ1a)
+               ={⊤}=∗
+               stateI σ1c
+               ∗ WP ec @ NotStuck; ⊤ {{ v, O ⤇ of_val v
+                    ∗ (∀ σ2c, stateI σ2c ={⊤,E}=∗ ∃ σ2a, source_state σ2a ∗ absr _ σ2a σ2c)}}
                                      ∗ (∀ σ2c, stateI σ2c ={⊤,E}=∗ φinv σ2c)
         ∗
         □ (∀ `{Hinv : invG Σ} `{Hcfg: cfgG OpTa Λa Σ} σ1c σ1c'
@@ -56,15 +278,15 @@ Theorem wp_recovery_crash_refinement {T R} OpTa OpTc Σ (Λa: Layer OpTa) (Λc: 
                let _ : irisG OpTc Λc Σ := IrisG _ _ _ Hinv stateI in
                stateI σ1c'
                ∗ WP rec @ NotStuck; ⊤ {{ v, (∀ σ2c, stateI σ2c ={⊤,E}=∗
-                   ∃ σ2a σ2a', source_state σ2a ∗ ⌜Λa.(crash_step) σ2a (Val σ2a' tt)
-                               ∧ absr σ2a' (Val σ2c tt)⌝)}}
+                   ∃ σ2a σ2a', source_state σ2a ∗ ⌜Λa.(crash_step) σ2a (Val σ2a' tt) ⌝ ∗
+                               absr _ σ2a' σ2c)}}
                                      ∗ (∀ σ2c, stateI σ2c ={⊤,E}=∗ φinv σ2c)))))%I) →
-  crash_refines absr Λc ec (rec_singleton rec) (Λa.(exec) ea)
+  crash_refines (absr_to_iProp absr) Λc ec (rec_singleton rec) (Λa.(exec) ea)
                 (and_then (Λa.(exec_halt) ea) (fun _ => Λa.(crash_step))).
 Proof.
   intros Hsub Hwp.
   assert (Hno_fault_cut :
-            ∀ σ1a, ¬ (v <- exec Λa ea; _ <- absr; pure v) σ1a Err ->
+            ∀ σ1a, ¬ (v <- exec Λa ea; _ <- (absr_to_iProp absr); pure v) σ1a Err ->
                    ¬ exec Λa ea σ1a Err).
   { clear. intros σ1a Hno_err.
     intros Hexec. apply Hno_err.
@@ -72,27 +294,32 @@ Proof.
   }
   assert (Hno_fault_cut':
             ∀ σ1a, ¬ (v <- _ <- exec_halt Λa ea;
-                          Λa.(crash_step); _ <- absr; pure v) σ1a Err ->
+                          Λa.(crash_step); _ <- (absr_to_iProp absr); pure v) σ1a Err ->
                    ¬ exec Λa ea σ1a Err).
   { clear. intros σ1a Hno_err.
     intros Hexec. apply Hno_err. do 3 left. apply exec_partial_err_exec_err; eauto.
   }
   assert (Hadeq: ∀ σ1a σ1c (Hno_fault : ¬  exec Λa ea σ1a Err),
-             absr σ1a (Val σ1c tt) → recv_adequate NotStuck ec rec σ1c
-                          (λ v' σ2c', ∃ σ2a, exec Λa ea σ1a (Val σ2a (existT _ v')) ∧
-                                             absr σ2a (Val σ2c' tt))
-                          (λ σ2c', ∃ tp2 σ2a σ3a, exec_partial Λa ea σ1a (Val σ2a tp2) ∧
-                                                   crash_step Λa σ2a (Val σ3a tt) ∧
-                                                   absr σ3a (Val σ2c' tt))).
-  { intros σ1a σ1c ? Habsr_init.
-    eapply wp_recovery_adequacy with
-        (φinv0 := fun σ => (∃ _ : cfgG Σ, φinv _ σ ∗ source_inv [existT T ea] σ1a)%I); eauto.
+             (absr_to_iProp absr σ1a (Val σ1c tt)) →
+             recv_adequate_internal (Σ := Σ) NotStuck ec rec σ1c
+                          (λ v' σ2c', ∃ H σ2a, ⌜ exec Λa ea σ1a (Val σ2a (existT _ v')) ⌝ ∗
+                                             absr H σ2a σ2c')%I
+                          (λ σ2c', ∃ H tp2 σ2a σ3a, ⌜ exec_partial Λa ea σ1a (Val σ2a tp2) ∧
+                                                      crash_step Λa σ2a (Val σ3a tt) ⌝ ∗
+                                                   absr H σ3a σ2c')%I).
+  { intros σ1a σ1c ? (k&Habsr_init).
+    eapply wp_recovery_adequacy_internal with
+        (φinv0 := fun σ => (∃ _ : cfgG Σ, φinv _ σ ∗ source_inv [existT T ea] σ1a)%I)
+        (k0 := k); eauto.
     iIntros (Hinv).
     assert (Inhabited Λa.(State)).
     { eexists; eauto. }
+    iPoseProof Habsr_init as "Habsr_init".
+    iApply (bupd_iter_mono with "[] Habsr_init"). iClear "Habsr_init".
+    iIntros "Habsr_init".
     iMod (source_cfg_init [existT _ ea] σ1a) as (cfgG) "(#Hsrc&Hpool&HstateA)"; auto.
     { intros Herr; apply Hno_fault. apply exec_partial_err_exec_err; eauto. }
-    iPoseProof (Hwp _ _ Habsr_init $! Hinv cfgG) as "H".
+    iPoseProof (Hwp _ _ with "Habsr_init") as "H".
     iMod "H" as (stateI) "Hwand"; eauto.
     iMod ("Hwand" with "[Hpool HstateA]") as "[Hstate [H [Hinv #Hφ]]]"; eauto.
     { iFrame. iFrame "#".
@@ -102,7 +329,7 @@ Proof.
     iSplitL "H"; last iSplitL "Hinv".
     * iApply wp_wand_l; iFrame "H". iIntros (v') "[Hmapsto Hopen]".
       iIntros (σ2c') "Hstate".
-      iMod ("Hopen" with "Hstate") as (σ2a) "(Hstate&%)".
+      iMod ("Hopen" with "Hstate") as (σ2a) "(Hstate&Habsr)".
       iInv "Hsrc" as (tp' σ') ">[Hauth Hp]" "_".
       iDestruct "Hp" as %Hp. destruct Hp as (Hp&Hno_fault'). rewrite //= in Hp.
       iDestruct (source_state_reconcile with "Hstate Hauth") as %Hstate; subst.
@@ -110,7 +337,7 @@ Proof.
       apply take_drop_middle in Hlookup.
 
       iApply fupd_mask_weaken; first by set_solver+.
-      iPureIntro. exists σ'; split; eauto.
+      iExists _, σ'. iSplit; auto. iPureIntro. 
       rewrite -Hlookup //= /of_val in Hp.
       eapply exec_partial_finish; eauto.
     * iIntros. iMod ("Hinv" with "[$]").
@@ -128,14 +355,14 @@ Proof.
       ** iApply wp_wand_l; iFrame.
          iIntros (_) "H1".
          iIntros (σ) "Hstate".
-         iMod ("H1" with "[$]") as (σ2a σ3a) "(Hstate&Hp)".
-         iDestruct "Hp" as %(Hcrash&Habsr).
+         iMod ("H1" with "[$]") as (σ2a σ3a) "(Hstate&Hp&Habsr)".
+         iDestruct "Hp" as %Hcrash.
          iMod (inv_open_timeless with "cfgInv") as "(Hinv&_)"; first by eassumption.
          iApply fupd_mask_weaken; auto.
          { set_solver+. }
          iDestruct "Hinv" as (tp' σ3a') "(Hauth&%&%)".
          iDestruct (source_state_reconcile with "Hstate Hauth") as %Hstate; subst.
-         iPureIntro. eexists _, _, _. intuition; eauto.
+         iExists _, _, _, _. iFrame. iPureIntro; intuition eauto.
       ** iIntros. iMod ("Hinv" with "[$]").
          iMod (inv_open_timeless with "cfgInv") as "(?&_)"; first by eassumption.
          iApply fupd_mask_weaken; auto.
@@ -149,9 +376,8 @@ Proof.
     {
       intros Hfalse; exfalso.
       destruct Hfalse as [|([]&?&?&?)]; eauto.
-      { eapply Habsr_no_err; eauto. }
       edestruct Hadeq; eauto.
-      eapply recv_adequate_not_stuck; eauto.
+      eapply recv_adequate_internal_not_stuck; eauto.
       apply exec_err_rexec_err; eauto.
     }
     intros ([]&σ1c&Habsr&Hexec).
@@ -345,3 +571,4 @@ Proof.
   destruct ret as [? []|]; eauto.
   exfalso. eapply recv_adequate_not_stuck; eauto using rexec_partial_err_rexec_err.
 Qed.
+*)
